\chapter{Kinematics}
\label{chapter:Kinematics}

%&& a &= b & \text{Proof \ref{proof:}} \label{equation:}

Topics:

different frames

deformation map

all the different kinds of tensors

material and spatial fields

derivatives of material and spatial fields

\section{Kinematic Variables}

\begin{itemize}
	\item $\vb{U} = \vb{U}(\vb{X}, t)$: displacement in material frame
	\begin{itemize}
		\item $\vb{U} := \vb*{\phi}_{t} - \vb{X}$
	\end{itemize}
	\item $\vb{u} = \vb{u}(\vb{x}, t)$: displacement in spatial frame
	\begin{itemize}
		\item $\vb{u} := \vb{U} \circ \vb*{\phi}_{t}^{-1} = \vb{x} - \vb*{\phi}_{t}^{-1}$
	\end{itemize}
	\item $\vb{V} = \vb{V}(\vb{X}, t)$: displacement in material frame
	\begin{itemize}
		\item $\vb{U} := \vb*{\phi}_{t} - \vb{X}$
	\end{itemize}
	\item $\vb{u} = \vb{u}(\vb{x}, t)$: displacement in spatial frame
	\begin{itemize}
		\item $\vb{u} := \vb{U} \circ \vb*{\phi}_{t}^{-1} = \vb{x} - \vb*{\phi}_{t}^{-1}$
	\end{itemize}
\end{itemize}

\begin{table}
	
\end{table}